{"nbformat":4,"nbformat_minor":0,"metadata":{"colab":{"provenance":[],"authorship_tag":"ABX9TyPTPGee8cH66OOpX7Q/qq2N"},"kernelspec":{"name":"python3","display_name":"Python 3"},"language_info":{"name":"python"}},"cells":[{"cell_type":"markdown","source":["# Complete 100 Differential Equations Problem Set\n","\n","## I. Basic Concepts & Slope Fields (1–10)\n","1. Identify order and degree of $$y'' + 3y' + 2y = 0$$  \n","2. Sketch slope field for $$y' = x + y$$  \n","3. Sketch slope field for $$y' = y(1 - y)$$  \n","4. Determine if $$y = e^{-x}$$ satisfies $$y' + y = 0$$  \n","5. Determine if $$y = x^2 + 1$$ satisfies $$y' = 2x$$  \n","6. Plot isoclines for $$y' = x - y$$  \n","7. Verify $$y = Ce^{2x}$$ is a family of solutions to $$y' = 2y$$  \n","8. Verify $$y = Cx^3$$ solves $$xy' - 3y = 0$$  \n","9. Find general solution to $$y' = 0$$  \n","10. Find general solution to $$y' = k,$$ where \\(k\\) is constant  \n","\n","---\n","\n","## II. Separable Equations (11–25)\n","11. $$y' = xy$$  \n","12. $$y' = y(1 - y)$$  \n","13. $$y' = x^2y^3$$  \n","14. $$y' = \\frac{x}{1 + y^2}$$  \n","15. $$y' = \\sin x \\cos y$$  \n","16. $$y' = e^{x + y}$$  \n","17. $$y' = \\frac{y}{x}$$  \n","18. $$y' = (x^2 + 1)y^2$$  \n","19. $$y' = \\frac{2xy}{x^2 - 1}$$  \n","20. $$y' = \\frac{1 - y^2}{1 + x^2}$$  \n","21. $$y' = y\\ln y$$  \n","22. $$y' = \\frac{x^3}{y^2}$$  \n","23. $$y' = (1 + x^2)(1 + y^2)$$  \n","24. $$y' = \\frac{ye^x}{x}$$  \n","25. $$y' = \\frac{y}{x + y}$$  \n","\n","---\n","\n","## III. Linear First-Order Equations (26–40)\n","26. $$y' + y = e^x$$  \n","27. $$y' - 2y = 0$$  \n","28. $$y' + 3y = 6$$  \n","29. $$y' + \\frac{y}{x} = 1$$  \n","30. $$y' - \\frac{2y}{x} = x^2$$  \n","31. $$y' + 2xy = 3x^2$$  \n","32. $$y' + y\\tan x = \\sin x$$  \n","33. $$y' + \\frac{y}{x} = e^x$$  \n","34. $$y' + 2y = e^{-x}$$  \n","35. $$y' - 4y = 2e^{3x}$$  \n","36. $$y' + y\\ln x = x$$  \n","37. $$y' - y\\sec x = \\tan x$$  \n","38. $$y' + \\frac{2y}{x} = \\sin x$$  \n","39. $$y' + y = x e^{-x}$$  \n","40. $$y' + 2xy = \\cos x$$  \n","\n","---\n","\n","## IV. Exact & Integrating Factor Methods (41–50)\n","41. $$(2xy + y^2)\\,dx + (x^2 + 2xy)\\,dy = 0$$  \n","42. $$(3x^2 + y)\\,dx + (x + 2y)\\,dy = 0$$  \n","43. $$(y + 2x)\\,dx + (x + 3y)\\,dy = 0$$  \n","44. $$(y^2 - 2x)\\,dx + (2y - x^2)\\,dy = 0$$  \n","45. $$(2x + y)\\,dx + (x + 2y)\\,dy = 0$$  \n","46. $$(y^2 + xy)\\,dx + x^2\\,dy = 0$$  \n","47. $$(x + y)\\,dx + (y - x)\\,dy = 0$$  \n","48. $$(2xy - y^2)\\,dx + (x^2 - 2xy)\\,dy = 0$$  \n","49. $$(3x^2 + 2y)\\,dx + (2x + 3y^2)\\,dy = 0$$  \n","50. $$(y + e^x)\\,dx + (x + e^y)\\,dy = 0$$  \n","\n","---\n","\n","## V. Homogeneous & Bernoulli Equations (51–60)\n","51. $$y' = \\frac{y}{x} + \\frac{x^2}{y}$$  \n","52. $$y' = \\frac{x + y}{x - y}$$  \n","53. $$y' = \\frac{xy + y^2}{x^2}$$  \n","54. $$y' = \\frac{x^2 + y^2}{xy}$$  \n","55. $$y' = \\frac{y - x}{y + x}$$  \n","56. $$y' + \\frac{y}{x} = \\frac{1}{x^2}$$  \n","57. $$y' + \\frac{y}{x} = x^2$$  \n","58. $$y' + y = y^2$$  \n","59. $$y' + y = y^n$$  \n","60. $$y' + 3y = y^2 e^{2x}$$  \n","\n","---\n","\n","## VI. Second-Order Linear Homogeneous (61–75)\n","61. $$y'' = 0$$  \n","62. $$y'' + y = 0$$  \n","63. $$y'' - y = 0$$  \n","64. $$y'' + 4y' + 4y = 0$$  \n","65. $$y'' + 5y' + 6y = 0$$  \n","66. $$y'' - 3y' + 2y = 0$$  \n","67. $$y'' + 9y = 0$$  \n","68. $$y'' - 2y' + y = 0$$  \n","69. $$y'' + 2y' + 5y = 0$$  \n","70. $$y'' + y' - 6y = 0$$  \n","71. $$y'' - 4y = 0$$  \n","72. $$y'' + 16y = 0$$  \n","73. $$y'' + 2y' + y = 0$$  \n","74. $$y'' - 2y' + 10y = 0$$  \n","75. $$y'' + 4y' + 5y = 0$$  \n","\n","---\n","\n","## VII. Second-Order Non-Homogeneous (76–85)\n","76. $$y'' + y = \\sin x$$  \n","77. $$y'' + 4y = 8\\sin(2x)$$  \n","78. $$y'' - y = e^x$$  \n","79. $$y'' + y = e^{2x}$$  \n","80. $$y'' - 3y' + 2y = e^{2x}$$  \n","81. $$y'' + 9y = 3\\cos(3x)$$  \n","82. $$y'' + 2y' + y = x$$  \n","83. $$y'' - 4y = 2e^{2x}$$  \n","84. $$y'' + 2y' + 10y = 5\\sin(3x)$$  \n","85. $$y'' - y = \\cosh x$$  \n","\n","---\n","\n","## VIII. Applications to Modeling (86–95)\n","86. Exponential growth: $$\\frac{dy}{dt} = ky$$  \n","87. Radioactive decay: $$\\frac{dN}{dt} = -kN$$  \n","88. Newton’s cooling law: $$\\frac{dT}{dt} = -k(T - T_s)$$  \n","89. Logistic growth: $$\\frac{dP}{dt} = rP\\left(1 - \\frac{P}{K}\\right)$$  \n","90. Falling body: $$m\\frac{dv}{dt} = mg - kv$$  \n","91. RC circuit: $$\\frac{dq}{dt} + \\frac{1}{RC}q = E$$  \n","92. RL circuit: $$L\\frac{di}{dt} + Ri = E_0\\sin(\\omega t)$$  \n","93. Damped spring: $$m x'' + c x' + kx = 0$$  \n","94. Driven harmonic oscillator: $$x'' + \\omega^2x = F_0\\cos(\\omega t)$$  \n","95. Mixing problem: tank inflow/outflow model  \n","\n","---\n","\n","## IX. Systems of Differential Equations (96–100)\n","96. $$x' = x + y,\\quad y' = x - y$$  \n","97. $$x' = 2x - y,\\quad y' = x + 3y$$  \n","98. $$x' = 3x + 4y,\\quad y' = -4x + 3y$$  \n","99. $$x' = -y,\\quad y' = x$$  \n","100. $$x'' + y'' = -x - y$$  \n"],"metadata":{"id":"6oC9YSIxy_nB"}}]}
