{"nbformat":4,"nbformat_minor":0,"metadata":{"colab":{"provenance":[],"authorship_tag":"ABX9TyNYURp88wpGRO3XFe6z4Lyu"},"kernelspec":{"name":"python3","display_name":"Python 3"},"language_info":{"name":"python"}},"cells":[{"cell_type":"markdown","source":["# Phase 2 — Core Derivative Rules\n","\n","---\n","\n","## 1️⃣ Power Rule\n","\n","If \\( f(x) = x^n \\), then  \n","$$\n","\\boxed{f'(x) = n x^{n-1}}\n","$$\n","\n","Works for all real \\( n \\) — positive, negative, or fractional.\n","\n","**Examples**\n","$$\n","f(x) = x^3 \\Rightarrow f'(x) = 3x^2\n","$$\n","$$\n","f(x) = x^{-2} \\Rightarrow f'(x) = -2x^{-3}\n","$$\n","$$\n","f(x) = \\sqrt{x} = x^{1/2} \\Rightarrow f'(x) = \\tfrac{1}{2}x^{-1/2} = \\frac{1}{2\\sqrt{x}}\n","$$\n","\n","---\n","\n","## 2️⃣ Constant Rule & Constant Multiple Rule\n","\n","$$\n","\\frac{d}{dx}(c) = 0\n","$$\n","\n","$$\n","\\frac{d}{dx}[c\\,f(x)] = c\\,f'(x)\n","$$\n","\n","**Examples**\n","$$\n","\\frac{d}{dx}(7) = 0\n","$$\n","$$\n","\\frac{d}{dx}(5x^3) = 5 \\cdot 3x^2 = 15x^2\n","$$\n","\n","---\n","\n","## 3️⃣ Sum and Difference Rule\n","\n","$$\n","\\frac{d}{dx}[f(x) \\pm g(x)] = f'(x) \\pm g'(x)\n","$$\n","\n","**Example**\n","$$\n","\\frac{d}{dx}(x^3 + 4x^2 - 7x) = 3x^2 + 8x - 7\n","$$\n","\n","---\n","\n","## 4️⃣ Product Rule\n","\n","When functions multiply:\n","$$\n","\\boxed{(fg)' = f'g + fg'}\n","$$\n","\n","**Example**\n","$$\n","f(x) = x^2, \\quad g(x) = \\sin x\n","$$\n","$$\n","f'(x) = 2x, \\quad g'(x) = \\cos x\n","$$\n","$$\n","\\Rightarrow (x^2 \\sin x)' = 2x\\sin x + x^2\\cos x\n","$$\n","\n","---\n","\n","## 5️⃣ Quotient Rule\n","\n","For a quotient \\( \\frac{f(x)}{g(x)} \\):\n","$$\n","\\boxed{\\left(\\frac{f}{g}\\right)' = \\frac{f'g - fg'}{g^2}}\n","$$\n","\n","**Example**\n","$$\n","f(x) = x^2, \\quad g(x) = x + 1\n","$$\n","$$\n","f'(x) = 2x, \\quad g'(x) = 1\n","$$\n","$$\n","\\Rightarrow \\left(\\frac{x^2}{x+1}\\right)' = \\frac{(2x)(x+1) - x^2(1)}{(x+1)^2}\n","= \\frac{x^2 + 2x}{(x+1)^2}\n","$$\n","\n","---\n","\n","## 6️⃣ Chain Rule\n","\n","For a composition \\( f(g(x)) \\):\n","$$\n","\\boxed{(f \\circ g)' = f'(g(x)) \\cdot g'(x)}\n","$$\n","\n","**Example**\n","$$\n","f(x) = (3x^2 + 1)^5\n","$$\n","Let \\( u = 3x^2 + 1 \\).  \n","Then \\( f(x) = u^5 \\Rightarrow f'(x) = 5u^4 \\cdot \\frac{du}{dx} = 5(3x^2 + 1)^4 \\cdot 6x = 30x(3x^2 + 1)^4\n","$$\n","\n","---\n","\n","## 7️⃣ Derivatives of Common Functions\n","\n","| Function | Derivative |\n","|-----------|-------------|\n","| \\( c \\) | \\( 0 \\) |\n","| \\( x^n \\) | \\( n x^{n-1} \\) |\n","| \\( e^x \\) | \\( e^x \\) |\n","| \\( a^x \\) | \\( a^x \\ln a \\) |\n","| \\( \\ln x \\) | \\( \\frac{1}{x} \\) |\n","| \\( \\sin x \\) | \\( \\cos x \\) |\n","| \\( \\cos x \\) | \\( -\\sin x \\) |\n","| \\( \\tan x \\) | \\( \\sec^2 x \\) |\n","| \\( \\sec x \\) | \\( \\sec x \\tan x \\) |\n","| \\( \\csc x \\) | \\( -\\csc x \\cot x \\) |\n","| \\( \\cot x \\) | \\( -\\csc^2 x \\) |\n","\n","---\n","\n","## 8️⃣ Combined Example\n","\n","Differentiate:\n","$$\n","y = e^{3x}\\sin(2x)\n","$$\n","\n","**Solution**\n","\n","Use product + chain rules:\n","$$\n","y' = e^{3x}(3\\sin(2x) + 2\\cos(2x))\n","$$\n","\n","---\n","\n","## 9️⃣ Summary Sheet\n","\n","| Rule | Formula | Use When |\n","|-------|----------|-----------|\n","| Power | \\( n x^{n-1} \\) | \\( x^n \\) |\n","| Constant | \\( 0 \\) | constants |\n","| Constant Multiple | \\( c f'(x) \\) | constant × function |\n","| Sum/Diff | \\( f' \\pm g' \\) | addition/subtraction |\n","| Product | \\( f'g + fg' \\) | multiplication |\n","| Quotient | \\( \\frac{f'g - fg'}{g^2} \\) | division |\n","| Chain | \\( f'(g(x)) \\cdot g'(x) \\) | nested functions |\n","\n","---\n","\n","\n"],"metadata":{"id":"0a0yqrTwEQFH"}}]}