{"nbformat":4,"nbformat_minor":0,"metadata":{"colab":{"provenance":[],"authorship_tag":"ABX9TyMsj1tO4JMlz4HdeAyB1ng+"},"kernelspec":{"name":"python3","display_name":"Python 3"},"language_info":{"name":"python"}},"cells":[{"cell_type":"markdown","source":["# Problem 1 — Power Rule & Linearity (the true “baseline”)\n","\n","Differentiate:\n","\n","$$\n","f(x) = 2x^5 - 3x^3 + 4x - 9\n","$$\n","\n","---\n","\n","### Rules We’ll Use\n","\n","**Power Rule:**\n","$$\n","\\frac{d}{dx}x^n = n x^{n-1}\n","$$\n","\n","**Constant Multiple Rule:**\n","$$\n","\\frac{d}{dx}[c \\cdot g(x)] = c \\cdot g'(x)\n","$$\n","\n","**Sum/Difference Rule:**\n","Differentiate term-by-term.\n","\n","**Constant Rule:**\n","$$\n","\\frac{d}{dx}[c] = 0\n","$$\n","\n","---\n","\n","### Step-by-Step\n","\n","$$\n","\\frac{d}{dx}[2x^5] = 2 \\cdot 5x^4 = 10x^4\n","$$\n","\n","$$\n","\\frac{d}{dx}[-3x^3] = -3 \\cdot 3x^2 = -9x^2\n","$$\n","\n","$$\n","\\frac{d}{dx}[4x] = 4 \\cdot 1 = 4\n","$$\n","\n","$$\n","\\frac{d}{dx}[-9] = 0\n","$$\n","\n","---\n","\n","### Final Answer\n","\n","$$\n","f'(x) = 10x^4 - 9x^2 + 4\n","$$\n"],"metadata":{"id":"RBn1D0wYZHyJ"}},{"cell_type":"markdown","source":["# Problem 2 — Product Rule\n","\n","Differentiate:\n","\n","$$\n","g(x) = (x^2 + 1)(3x - 2)\n","$$\n","\n","---\n","\n","### Rule Reminder\n","\n","**Product Rule:**\n","$$\n","\\frac{d}{dx}[u \\cdot v] = u'v + uv'\n","$$\n","\n","where  \n","$$\n","u = (x^2 + 1), \\quad v = (3x - 2)\n","$$\n","\n","---\n","\n","### Step-by-Step\n","\n","Compute derivatives:\n","$$\n","u' = 2x\n","$$\n","$$\n","v' = 3\n","$$\n","\n","Apply the product rule:\n","$$\n","g'(x) = (2x)(3x - 2) + (x^2 + 1)(3)\n","$$\n","\n","Expand each term:\n","$$\n","g'(x) = (6x^2 - 4x) + (3x^2 + 3)\n","$$\n","\n","Simplify:\n","$$\n","g'(x) = 9x^2 - 4x + 3\n","$$\n","\n","---\n","\n","### Final Answer\n","\n","$$\n","g'(x) = 9x^2 - 4x + 3\n","$$\n"],"metadata":{"id":"bpfuQ5WkZ3L9"}},{"cell_type":"markdown","source":["# Problem 3 — Quotient Rule\n","\n","Differentiate:\n","\n","$$\n","h(x) = \\frac{x^2 + 1}{x - 3}\n","$$\n","\n","---\n","\n","### Rule Reminder\n","\n","If  \n","$$\n","h(x) = \\frac{u}{v},\n","$$  \n","then  \n","$$\n","h'(x) = \\frac{u'v - uv'}{v^2}\n","$$\n","\n","where  \n","$$\n","u = x^2 + 1, \\quad v = x - 3\n","$$\n","\n","---\n","\n","### Step-by-Step\n","\n","Compute derivatives:\n","$$\n","u' = 2x\n","$$\n","$$\n","v' = 1\n","$$\n","\n","Substitute into the rule:\n","$$\n","h'(x) = \\frac{(2x)(x - 3) - (x^2 + 1)(1)}{(x - 3)^2}\n","$$\n","\n","Expand the numerator:\n","$$\n","h'(x) = \\frac{(2x^2 - 6x) - (x^2 + 1)}{(x - 3)^2}\n","$$\n","\n","Simplify:\n","$$\n","h'(x) = \\frac{x^2 - 6x - 1}{(x - 3)^2}\n","$$\n","\n","---\n","\n","### Final Answer\n","\n","$$\n","h'(x) = \\frac{x^2 - 6x - 1}{(x - 3)^2}\n","$$\n"],"metadata":{"id":"5N63LbMUZ7uW"}},{"cell_type":"markdown","source":["# Problem 4 — Chain Rule\n","\n","Differentiate:\n","\n","$$\n","f(x) = (3x^2 + 2x + 1)^4\n","$$\n","\n","---\n","\n","### Rule Reminder\n","\n","If  \n","$$\n","y = [u(x)]^n,\n","$$  \n","then  \n","$$\n","\\frac{dy}{dx} = n [u(x)]^{n-1} \\cdot u'(x)\n","$$  \n","\n","This is the **Chain Rule** — multiply the derivative of the outer function by the derivative of the inner function.\n","\n","---\n","\n","### Step-by-Step\n","\n","Let the inner function:  \n","$$\n","u = 3x^2 + 2x + 1\n","$$  \n","Then:  \n","$$\n","u' = 6x + 2\n","$$\n","\n","The outer function is \\( u^4 \\), whose derivative is \\( 4u^3 \\).\n","\n","Now apply the rule:  \n","$$\n","f'(x) = 4(3x^2 + 2x + 1)^3 \\cdot (6x + 2)\n","$$\n","\n","Simplify:  \n","$$\n","f'(x) = (24x + 8)(3x^2 + 2x + 1)^3\n","$$\n","\n","Or equivalently (factored form):  \n","$$\n","f'(x) = 4(6x + 2)(3x^2 + 2x + 1)^3\n","$$\n","\n","---\n","\n","### Final Answer\n","\n","$$\n","f'(x) = (24x + 8)(3x^2 + 2x + 1)^3\n","$$\n"],"metadata":{"id":"1ALfw4_taT1K"}},{"cell_type":"code","source":[],"metadata":{"id":"r-d4NpnLaUOM"},"execution_count":null,"outputs":[]},{"cell_type":"markdown","source":["# Problem 5 — Product + Chain Rule\n","\n","Differentiate:\n","\n","$$\n","y = (x^2 + 1)^3 (2x - 5)^4\n","$$\n","\n","---\n","\n","### Setup (Product Rule)\n","\n","Let  \n","$$\n","u = (x^2 + 1)^3, \\quad v = (2x - 5)^4\n","$$\n","\n","Then  \n","$$\n","y' = u'v + uv'\n","$$\n","\n","---\n","\n","### Chain Pieces\n","\n","Compute \\( u' \\) using the **Chain Rule**:\n","$$\n","u' = 3(x^2 + 1)^2 \\cdot (2x) = 6x(x^2 + 1)^2\n","$$\n","\n","Compute \\( v' \\) using the **Chain Rule**:\n","$$\n","v' = 4(2x - 5)^3 \\cdot 2 = 8(2x - 5)^3\n","$$\n","\n","---\n","\n","### Assemble the Product Rule\n","\n","Substitute \\( u', v, u, v' \\):\n","\n","$$\n","y' = 6x(x^2 + 1)^2 (2x - 5)^4 + (x^2 + 1)^3 \\cdot 8(2x - 5)^3\n","$$\n","\n","---\n","\n","### Factor Common Terms\n","\n","$$\n","y' = (x^2 + 1)^2 (2x - 5)^3 [6x(2x - 5) + 8(x^2 + 1)]\n","$$\n","\n","Simplify inside the brackets:\n","$$\n","y' = (x^2 + 1)^2 (2x - 5)^3 [(12x^2 - 30x) + (8x^2 + 8)]\n","$$\n","\n","Combine like terms:\n","$$\n","y' = (x^2 + 1)^2 (2x - 5)^3 (20x^2 - 30x + 8)\n","$$\n","\n","---\n","\n","### Final Answer\n","\n","$$\n","y' = (x^2 + 1)^2 (2x - 5)^3 (20x^2 - 30x + 8)\n","$$\n"],"metadata":{"id":"ngFbgN9SaqAf"}},{"cell_type":"markdown","source":["# Problem 6 — Implicit Differentiation\n","\n","Given:\n","\n","$$\n","x^2 + y^2 = 25\n","$$\n","\n","We must find \\( \\frac{dy}{dx} \\).\n","\n","---\n","\n","### Step-by-Step\n","\n","Differentiate both sides with respect to \\( x \\), remembering that \\( y \\) is a function of \\( x \\):\n","\n","$$\n","\\frac{d}{dx}(x^2) + \\frac{d}{dx}(y^2) = \\frac{d}{dx}(25)\n","$$\n","\n","Differentiate term by term:\n","\n","$$\n","2x + 2y \\frac{dy}{dx} = 0\n","$$\n","\n","(because \\( \\frac{d}{dx}(y^2) = 2y \\frac{dy}{dx} \\) by the chain rule)\n","\n","---\n","\n","### Solve for \\( \\frac{dy}{dx} \\)\n","\n","$$\n","2y \\frac{dy}{dx} = -2x\n","$$\n","\n","Divide both sides by \\( 2y \\):\n","\n","$$\n","\\frac{dy}{dx} = -\\frac{x}{y}\n","$$\n","\n","---\n","\n","### Final Answer\n","\n","$$\n","\\frac{dy}{dx} = -\\frac{x}{y}\n","$$\n"],"metadata":{"id":"MPRVecgka4kJ"}},{"cell_type":"markdown","source":["# Problem 7 — Logarithmic Differentiation\n","\n","Differentiate:\n","\n","$$\n","y = x^x\n","$$\n","\n","---\n","\n","### Step 1: Take the Natural Log of Both Sides\n","\n","$$\n","\\ln y = \\ln(x^x)\n","$$\n","\n","Use the logarithmic identity \\( \\ln(a^b) = b \\ln a \\):\n","\n","$$\n","\\ln y = x \\ln x\n","$$\n","\n","---\n","\n","### Step 2: Differentiate Both Sides Implicitly with Respect to \\( x \\)\n","\n","$$\n","\\frac{1}{y} \\frac{dy}{dx} = 1 \\cdot \\ln x + x \\cdot \\frac{1}{x}\n","$$\n","\n","Simplify:\n","\n","$$\n","\\frac{1}{y} \\frac{dy}{dx} = \\ln x + 1\n","$$\n","\n","---\n","\n","### Step 3: Multiply Both Sides by \\( y \\)\n","\n","$$\n","\\frac{dy}{dx} = y (\\ln x + 1)\n","$$\n","\n","Substitute back \\( y = x^x \\):\n","\n","$$\n","\\frac{dy}{dx} = x^x (\\ln x + 1)\n","$$\n","\n","---\n","\n","### Final Answer\n","\n","$$\n","\\frac{dy}{dx} = x^x (\\ln x + 1)\n","$$\n"],"metadata":{"id":"1RcdYLJ3a9Lb"}},{"cell_type":"markdown","source":["# Problem 8 — Derivative of Exponential Function\n","\n","Differentiate:\n","\n","$$\n","f(x) = 5^{2x + 1}\n","$$\n","\n","---\n","\n","### Step 1: Recall the Rule\n","\n","For any base \\( a > 0 \\):\n","\n","$$\n","\\frac{d}{dx}\\left(a^{u(x)}\\right) = a^{u(x)} \\ln(a) \\cdot u'(x)\n","$$\n","\n","---\n","\n","### Step 2: Identify the Parts\n","\n","Here:\n","\n","$$\n","a = 5, \\quad u(x) = 2x + 1\n","$$\n","\n","Then:\n","\n","$$\n","u'(x) = 2\n","$$\n","\n","---\n","\n","### Step 3: Apply the Rule\n","\n","$$\n","f'(x) = 5^{2x + 1} \\ln(5) \\cdot 2\n","$$\n","\n","Simplify:\n","\n","$$\n","f'(x) = 2 \\ln(5) \\cdot 5^{2x + 1}\n","$$\n","\n","---\n","\n","### Final Answer\n","\n","$$\n","f'(x) = 2 \\ln(5) \\, 5^{2x + 1}\n","$$\n"],"metadata":{"id":"wQsx8fo5beSK"}},{"cell_type":"markdown","source":["# Problem 9 — Derivative of a Logarithmic Function\n","\n","Differentiate:\n","\n","$$\n","g(x) = \\ln(3x^2 - 2)\n","$$\n","\n","---\n","\n","### Step 1: Recall the Rule\n","\n","For any differentiable inner function \\( u(x) \\):\n","\n","$$\n","\\frac{d}{dx}[\\ln(u)] = \\frac{1}{u} \\cdot u'(x)\n","$$\n","\n","---\n","\n","### Step 2: Identify the Inner Function\n","\n","Let  \n","$$\n","u = 3x^2 - 2 \\quad \\Rightarrow \\quad u' = 6x\n","$$\n","\n","---\n","\n","### Step 3: Apply the Rule\n","\n","$$\n","g'(x) = \\frac{1}{3x^2 - 2} \\cdot 6x\n","$$\n","\n","Simplify:\n","\n","$$\n","g'(x) = \\frac{6x}{3x^2 - 2}\n","$$\n","\n","---\n","\n","### Final Answer\n","\n","$$\n","g'(x) = \\frac{6x}{3x^2 - 2}\n","$$\n"],"metadata":{"id":"HO7c2YRpbxge"}},{"cell_type":"markdown","source":["# Problem 10 — Derivative of a Trigonometric Function (with Chain Rule)\n","\n","Differentiate:\n","\n","$$\n","y = \\sin(2x + 3)\n","$$\n","\n","---\n","\n","### Step 1: Recall the Rule\n","\n","$$\n","\\frac{d}{dx}[\\sin(u)] = \\cos(u) \\cdot u'(x)\n","$$\n","\n","---\n","\n","### Step 2: Identify the Inner Function\n","\n","Let  \n","$$\n","u = 2x + 3 \\quad \\Rightarrow \\quad u' = 2\n","$$\n","\n","---\n","\n","### Step 3: Apply the Rule\n","\n","$$\n","y' = \\cos(2x + 3) \\cdot 2\n","$$\n","\n","Simplify:\n","\n","$$\n","y' = 2 \\cos(2x + 3)\n","$$\n","\n","---\n","\n","### Final Answer\n","\n","$$\n","y' = 2 \\cos(2x + 3)\n","$$\n"],"metadata":{"id":"uyf2X2FtcCwd"}},{"cell_type":"markdown","source":["# Problem 11 — Derivative of a Cosine Function (with Chain Rule)\n","\n","Differentiate:\n","\n","$$\n","y = \\cos(5x^2)\n","$$\n","\n","---\n","\n","### Step 1: Recall the Rule\n","\n","$$\n","\\frac{d}{dx}[\\cos(u)] = -\\sin(u) \\cdot u'(x)\n","$$\n","\n","---\n","\n","### Step 2: Identify the Inner Function\n","\n","Let  \n","$$\n","u = 5x^2 \\quad \\Rightarrow \\quad u' = 10x\n","$$\n","\n","---\n","\n","### Step 3: Apply the Rule\n","\n","$$\n","y' = -\\sin(5x^2) \\cdot 10x\n","$$\n","\n","Simplify:\n","\n","$$\n","y' = -10x \\sin(5x^2)\n","$$\n","\n","---\n","\n","### Final Answer\n","\n","$$\n","y' = -10x \\sin(5x^2)\n","$$\n"],"metadata":{"id":"9Mx7pElmcIhM"}},{"cell_type":"markdown","source":["# Problem 12 — Derivative of a Tangent Function (with Chain Rule)\n","\n","Differentiate:\n","\n","$$\n","y = \\tan(3x)\n","$$\n","\n","---\n","\n","### Step 1: Recall the Rule\n","\n","$$\n","\\frac{d}{dx}[\\tan(u)] = \\sec^2(u) \\cdot u'(x)\n","$$\n","\n","---\n","\n","### Step 2: Identify the Inner Function\n","\n","Let  \n","$$\n","u = 3x \\quad \\Rightarrow \\quad u' = 3\n","$$\n","\n","---\n","\n","### Step 3: Apply the Rule\n","\n","$$\n","y' = \\sec^2(3x) \\cdot 3\n","$$\n","\n","Simplify:\n","\n","$$\n","y' = 3\\sec^2(3x)\n","$$\n","\n","---\n","\n","### Final Answer\n","\n","$$\n","y' = 3\\sec^2(3x)\n","$$\n"],"metadata":{"id":"6Ys49RpjcXk5"}},{"cell_type":"markdown","source":["# Problem 13 — Derivative of an Inverse Trigonometric Function\n","\n","Differentiate:\n","\n","$$\n","y = \\arctan(x)\n","$$\n","\n","---\n","\n","### Step 1: Recall the Rule\n","\n","$$\n","\\frac{d}{dx}[\\arctan(u)] = \\frac{u'(x)}{1 + [u(x)]^2}\n","$$\n","\n","---\n","\n","### Step 2: Identify the Inner Function\n","\n","Let  \n","$$\n","u = x \\quad \\Rightarrow \\quad u' = 1\n","$$\n","\n","---\n","\n","### Step 3: Apply the Rule\n","\n","$$\n","y' = \\frac{1}{1 + x^2}\n","$$\n","\n","---\n","\n","### Final Answer\n","\n","$$\n","y' = \\frac{1}{1 + x^2}\n","$$\n"],"metadata":{"id":"io6zzrIWcsKJ"}},{"cell_type":"markdown","source":["# Problem 14 — Derivative of an Inverse Sine Function\n","\n","Differentiate:\n","\n","$$\n","y = \\arcsin(2x)\n","$$\n","\n","---\n","\n","### Step 1: Recall the Rule\n","\n","$$\n","\\frac{d}{dx}[\\arcsin(u)] = \\frac{u'(x)}{\\sqrt{1 - [u(x)]^2}}\n","$$\n","\n","---\n","\n","### Step 2: Identify the Inner Function\n","\n","Let  \n","$$\n","u = 2x \\quad \\Rightarrow \\quad u' = 2\n","$$\n","\n","---\n","\n","### Step 3: Apply the Rule\n","\n","$$\n","y' = \\frac{2}{\\sqrt{1 - (2x)^2}}\n","$$\n","\n","Simplify:\n","\n","$$\n","y' = \\frac{2}{\\sqrt{1 - 4x^2}}\n","$$\n","\n","---\n","\n","### Final Answer\n","\n","$$\n","y' = \\frac{2}{\\sqrt{1 - 4x^2}}\n","$$\n"],"metadata":{"id":"vXgnSMjLdaUM"}},{"cell_type":"markdown","source":["# Problem 15 — Derivative of an Inverse Cosine Function\n","\n","Differentiate:\n","\n","$$\n","y = \\arccos(3x)\n","$$\n","\n","---\n","\n","### Step 1: Recall the Rule\n","\n","$$\n","\\frac{d}{dx}[\\arccos(u)] = -\\frac{u'(x)}{\\sqrt{1 - [u(x)]^2}}\n","$$\n","\n","---\n","\n","### Step 2: Identify the Inner Function\n","\n","Let  \n","$$\n","u = 3x \\quad \\Rightarrow \\quad u' = 3\n","$$\n","\n","---\n","\n","### Step 3: Apply the Rule\n","\n","$$\n","y' = -\\frac{3}{\\sqrt{1 - (3x)^2}}\n","$$\n","\n","Simplify:\n","\n","$$\n","y' = -\\frac{3}{\\sqrt{1 - 9x^2}}\n","$$\n","\n","---\n","\n","### Final Answer\n","\n","$$\n","y' = -\\frac{3}{\\sqrt{1 - 9x^2}}\n","$$\n"],"metadata":{"id":"h9i0fnBCdi55"}},{"cell_type":"markdown","source":["# Problem 16 — Derivative of a Hyperbolic Sine Function\n","\n","Differentiate:\n","\n","$$\n","y = \\sinh(2x)\n","$$\n","\n","---\n","\n","### Step 1: Recall the Rule\n","\n","$$\n","\\frac{d}{dx}[\\sinh(u)] = \\cosh(u) \\cdot u'(x)\n","$$\n","\n","---\n","\n","### Step 2: Identify the Inner Function\n","\n","Let  \n","$$\n","u = 2x \\quad \\Rightarrow \\quad u' = 2\n","$$\n","\n","---\n","\n","### Step 3: Apply the Rule\n","\n","$$\n","y' = \\cosh(2x) \\cdot 2\n","$$\n","\n","Simplify:\n","\n","$$\n","y' = 2\\cosh(2x)\n","$$\n","\n","---\n","\n","### Final Answer\n","\n","$$\n","y' = 2\\cosh(2x)\n","$$\n"],"metadata":{"id":"7WrN_tlZd1aG"}},{"cell_type":"markdown","source":["# Problem 17 — Derivative of a Hyperbolic Cosine Function\n","\n","Differentiate:\n","\n","$$\n","y = \\cosh(3x)\n","$$\n","\n","---\n","\n","### Step 1: Recall the Rule\n","\n","$$\n","\\frac{d}{dx}[\\cosh(u)] = \\sinh(u) \\cdot u'(x)\n","$$\n","\n","---\n","\n","### Step 2: Identify the Inner Function\n","\n","Let  \n","$$\n","u = 3x \\quad \\Rightarrow \\quad u' = 3\n","$$\n","\n","---\n","\n","### Step 3: Apply the Rule\n","\n","$$\n","y' = \\sinh(3x) \\cdot 3\n","$$\n","\n","Simplify:\n","\n","$$\n","y' = 3\\sinh(3x)\n","$$\n","\n","---\n","\n","### Final Answer\n","\n","$$\n","y' = 3\\sinh(3x)\n","$$\n"],"metadata":{"id":"cpvh-krTeCNe"}},{"cell_type":"markdown","source":["# Problem 18 — Derivative of a Hyperbolic Tangent Function\n","\n","Differentiate:\n","\n","$$\n","y = \\tanh(x^2)\n","$$\n","\n","---\n","\n","### Step 1: Recall the Rule\n","\n","$$\n","\\frac{d}{dx}[\\tanh(u)] = \\sech^2(u) \\cdot u'(x)\n","$$\n","\n","where  \n","$$\n","\\sech(u) = \\frac{1}{\\cosh(u)}.\n","$$\n","\n","---\n","\n","### Step 2: Identify the Inner Function\n","\n","Let  \n","$$\n","u = x^2 \\quad \\Rightarrow \\quad u' = 2x\n","$$\n","\n","---\n","\n","### Step 3: Apply the Rule\n","\n","$$\n","y' = \\sech^2(x^2) \\cdot 2x\n","$$\n","\n","Simplify:\n","\n","$$\n","y' = 2x \\sech^2(x^2)\n","$$\n","\n","---\n","\n","### Final Answer\n","\n","$$\n","y' = 2x \\sech^2(x^2)\n","$$\n"],"metadata":{"id":"8uML8vbdeMdt"}},{"cell_type":"markdown","source":["# Problem 19 — Higher-Order Derivatives\n","\n","Given:\n","\n","$$\n","f(x) = x^3 - 6x^2 + 9x + 1\n","$$\n","\n","We will find the **first** and **second** derivatives.\n","\n","---\n","\n","### Step 1: First Derivative \\( f'(x) \\)\n","\n","Differentiate term-by-term:\n","\n","$$\n","f'(x) = 3x^2 - 12x + 9\n","$$\n","\n","---\n","\n","### Step 2: Second Derivative \\( f''(x) \\)\n","\n","Differentiate \\( f'(x) \\):\n","\n","$$\n","f''(x) = 6x - 12\n","$$\n","\n","---\n","\n","### Final Results\n","\n","$$\n","f'(x) = 3x^2 - 12x + 9\n","$$\n","\n","$$\n","f''(x) = 6x - 12\n","$$\n","\n","---\n","\n","### Interpretation\n","\n","- \\( f'(x) \\): Represents the **slope** or **rate of change** of \\( f(x) \\).\n","- \\( f''(x) \\): Represents the **curvature** or **concavity** of \\( f(x) \\).  \n","  - \\( f''(x) > 0 \\) ⇒ Concave up  \n","  - \\( f''(x) < 0 \\) ⇒ Concave down\n"],"metadata":{"id":"VPK4eglae5F1"}},{"cell_type":"markdown","source":["# Problem 20 — Critical Points & Local Extrema\n","\n","Function:\n","$$\n","f(x) = x^3 - 3x^2 - 9x + 5\n","$$\n","\n","---\n","\n","## 1) First Derivative & Critical Points\n","Compute \\( f'(x) \\):\n","$$\n","f'(x) = 3x^2 - 6x - 9 = 3(x^2 - 2x - 3) = 3(x-3)(x+1).\n","$$\n","\n","Set \\( f'(x) = 0 \\) to find critical points:\n","$$\n","3(x-3)(x+1)=0 \\;\\;\\Rightarrow\\;\\; x=-1,\\; x=3.\n","$$\n","\n","---\n","\n","## 2) Second Derivative Test\n","Compute \\( f''(x) \\):\n","$$\n","f''(x) = 6x - 6 = 6(x-1).\n","$$\n","\n","At \\( x=-1 \\):\n","$$\n","f''(-1) = 6(-1) - 6 = -12 < 0 \\;\\Rightarrow\\; \\text{local maximum}.\n","$$\n","Function value:\n","$$\n","f(-1) = (-1)^3 - 3(-1)^2 - 9(-1) + 5 = -1 - 3 + 9 + 5 = 10.\n","$$\n","Local max at \\( (-1,\\,10) \\).\n","\n","At \\( x=3 \\):\n","$$\n","f''(3) = 6(3) - 6 = 12 > 0 \\;\\Rightarrow\\; \\text{local minimum}.\n","$$\n","Function value:\n","$$\n","f(3) = 27 - 27 - 27 + 5 = -22.\n","$$\n","Local min at \\( (3,\\,-22) \\).\n","\n","---\n","\n","## 3) (Optional) Increasing/Decreasing Intervals\n","Using \\( f'(x) = 3(x-3)(x+1) \\):\n","- Increasing on \\( (-\\infty,-1) \\) and \\( (3,\\infty) \\).\n","- Decreasing on \\( (-1,3) \\).\n"],"metadata":{"id":"JDX3_SsHe9K-"}},{"cell_type":"markdown","source":["# Problem 21 — Concavity & Inflection\n","\n","Function:\n","$$\n","f(x) = x^3 - 3x^2 - 9x + 5\n","$$\n","\n","---\n","\n","## 1) Second Derivative\n","$$\n","f''(x) = 6x - 6 = 6(x - 1)\n","$$\n","\n","---\n","\n","## 2) Concavity Intervals\n","Concave up where \\( f''(x) > 0 \\):\n","$$\n","6(x-1) > 0 \\;\\;\\Longleftrightarrow\\;\\; x > 1\n","$$\n","So, concave up on \\( (1,\\infty) \\).\n","\n","Concave down where \\( f''(x) < 0 \\):\n","$$\n","6(x-1) < 0 \\;\\;\\Longleftrightarrow\\;\\; x < 1\n","$$\n","So, concave down on \\( (-\\infty,1) \\).\n","\n","---\n","\n","## 3) Inflection Point(s)\n","Solve \\( f''(x) = 0 \\):\n","$$\n","6(x-1)=0 \\;\\;\\Longrightarrow\\;\\; x=1\n","$$\n","Sign changes from negative to positive across \\( x=1 \\) \\( \\Rightarrow \\) valid inflection point.\n","\n","Evaluate \\( f(1) \\):\n","$$\n","f(1) = 1 - 3 - 9 + 5 = -6\n","$$\n","\n","**Inflection point:** \\( (1,-6) \\).\n"],"metadata":{"id":"aOwOifLOfWPq"}},{"cell_type":"markdown","source":["# Problem 22 — Optimization (Maximum Product with Fixed Sum)\n","\n","**Question:** Find two positive numbers whose sum is 20 and whose product is as large as possible.\n","\n","Let the numbers be \\( x \\) and \\( 20 - x \\) with \\( 0 < x < 20 \\).\n","\n","**Product function:**\n","$$\n","P(x) = x(20 - x) = 20x - x^2\n","$$\n","\n","**Differentiate:**\n","$$\n","P'(x) = 20 - 2x\n","$$\n","\n","**Critical point (set derivative to zero):**\n","$$\n","P'(x)=0 \\;\\Longrightarrow\\; 20 - 2x = 0 \\;\\Longrightarrow\\; x = 10\n","$$\n","Then the other number is \\( 20 - 10 = 10 \\).\n","\n","**Second derivative test:**\n","$$\n","P''(x) = -2 < 0 \\;\\Longrightarrow\\; \\text{local (and global) maximum on } (0,20).\n","$$\n","\n","**Answer:** The two numbers are \\( 10 \\) and \\( 10 \\), with maximum product\n","$$\n","P_{\\max} = 10 \\cdot 10 = 100.\n","$$\n"],"metadata":{"id":"lh4KcJR_faXz"}}]}